theories/L/TM/TMunflatten.v
@@ -3,6 +3,7 @@ Require Import PslBase.FiniteTypes.
 From PslBase.FiniteTypes Require Import VectorFin Cardinality.
 
 From Undecidability Require Import L.TM.TMflat.
+From Undecidability Require L.TM.TMEncoding.
 
 
 Definition Vector_of_list_length A n (l:list A) : option (Vector.t A n) :=
@@ -20,12 +21,6 @@ Proof.
   f_equal.
   rewrite <- Eqdep_dec.eq_rect_eq_dec. easy. decide equality.
 Qed.
-(*
-Definition Fin_of_nat_try n i : option (Fin.t n) :=
-  match Fin.of_nat i n with
-    inleft x => Some x
-  | _ => None
-  end.*)
 
 Definition unflatten_symb (sig:finType)  (i:option nat): option sig:=
   match i with
@@ -46,22 +41,12 @@ Definition unflatten_acts (sig:finType) n (l__r : list (option nat * move)) : (V
 Definition unflatten_trans (states:finType) (sig:finType) d n (f:list (nat * list (option nat) * (nat * list (option nat * move))))
   : states * Vector.t (option sig) n -> states * Vector.t (option sig * move) n :=
   fun '(st,l) =>
-    let (st__o,l__r) := lookup f (index st,map (option_map (fun x => index x)) (Vector.to_list l)) (0,[]) in
-    (nth st__o (elem _) d, unflatten_acts sig n l__r)
-.
+    let (st__o,l__r) := lookup f (index st,map (option_map (fun x => index x)) (Vector.to_list l)) (index st,repeat (None,N) n) in
+    (nth st__o (elem _) d, unflatten_acts sig n l__r).
 
 
 Definition unflatten_halt states (f: list bool) (i : (Fin.t states)) : bool :=
   nth (index i) f false.
-(*
-Definition from_mTM sig n (M:mTM sig n) : TM :=
-  {| sig := Cardinality sig ;
-     tapes := n;
-     states := Cardinality (TM.states M);
-     trans := flatten_trans (@TM.trans _ _ M);
-     start := index (TM.start M);
-     halt := flatten_halt (@TM.halt _ _ M);
-  |}.*)
 
 Local Definition def n : Fin.t (max 1 n).
 Proof.
@@ -107,8 +92,6 @@ Proof.
   unfold Cardinality.
   destruct (elem X). cbn. intros. omega. easy.
 Qed.
-  
-
 
 Definition unflatten_in (sig:finType) n (l__r : list (option nat)) : (Vector.t (option sig) n) :=
   match Vector_of_list_length n  (map (unflatten_symb sig) l__r) with
@@ -139,32 +122,35 @@ Proof.
   -rewrite map_length. easy.
 Qed.
 
-Record validFlatTrans (states sig n:nat) (f:list (nat * list (option nat) * (nat * list (option nat * move)))) : Prop :=
+Record validFlatTrans (sig n states:nat) (f:list (nat * list (option nat) * (nat * list (option nat * move)))) : Prop :=
   {
     flatTrans_inj:
       (forall a' b1 b2 , (a', b1) el f -> (a', b2) el f -> b1 = b2);
-    flatTrans_tot:
-      (forall s v, (exists r, ((s,v),r) el f)  <-> s < states
-                                       /\ length v = n
-                                       /\ forall a, Some a el v -> a < sig);
-    flatTrans_res_ok: forall x s' v',
-        (x,(s',v')) el f
-        -> s' < states
+    flatTrans_bound: forall s s' v v',
+        ((s,v),(s',v')) el f
+        -> s < states
+          /\ length v = n
+          /\ (forall a, Some a el v -> a < sig)
+          /\ s' < states
           /\ length v' = n
           /\ (forall a m, (Some a,m) el v' -> a < sig)   
   }.
 
-Lemma flatTrans_in_ok states sig n f:
-  validFlatTrans states sig n f ->
-  forall s v r,
-  ((s,v),r) el f
-  -> s < states
-    /\ length v = n
-    /\ (forall a, Some a el v -> a < sig).
-Proof.
-  intros H s v r ?.
-  eapply flatTrans_tot. all:eauto.
-Qed. 
+Definition validFlatTM (M:TM) :=
+  validFlatTrans M.(sig) M.(tapes) M.(states) M.(trans)
+  /\ M.(start) < M.(states).
+
+(* Lemma flatTrans_in_ok states sig n f: *)
+(*   validFlatTrans sig n states f -> *)
+(*   forall s v r, *)
+(*   ((s,v),r) el f *)
+(*   -> s < states *)
+(*     /\ length v = n *)
+(*     /\ (forall a, Some a el v -> a < sig). *)
+(* Proof. *)
+(*   intros H s v r ?. *)
+(*   eapply flatTrans_tot. all:eauto. *)
+(* Qed.  *)
 (*
 
 Lemma isFlattening_inv sig n (M':mTM sig n) d trans0 s s' v v':
@@ -207,47 +193,69 @@ Proof.
   induction l;cbn. easy. rewrite IHl at 1. reflexivity.
 Qed.
 
+Lemma lookup_sound' (A: eqType) (B: Type) (L : list (prod A B)) a b def :
+  (forall a' b1 b2, (a',b1) el L -> (a',b2) el L -> b1=b2) -> ( (a,b) el L \/ ((forall b', ~ (a,b') el L) /\ b = def) ) -> lookup L a def = b.
+Proof.
+  intros H1 H2. unfold lookup.
+  destruct filter eqn:E.
+  - destruct H2 as [H2|H2].
+    +assert ((a,b) el filter (fun p : A * B => Dec (fst p = a)) L) by ( rewrite in_filter_iff ; eauto).
+     now rewrite E in H.
+    +easy.
+  - destruct p. assert ((e,b0) el (filter (fun p : A * B => Dec (fst p = a)) L)) by now rewrite E.
+    rewrite in_filter_iff in H. 
+    dec; cbn in *; subst; firstorder.
+Qed.
+
 Lemma unflatten_trans_correct st sig n d trans0:
-  validFlatTrans st sig n trans0
+  validFlatTrans sig n st trans0
   -> isFlatteningTransOf trans0 (unflatten_trans (sig:=finType_CS (Fin.t sig)) (states := finType_CS (Fin.t st)) (n:=n) d trans0).
 Proof.
   intros H.
-  econstructor;split.
-  -intros H'.
+  split.
+  -intros ? ? ? ? H'.
    eexists (nth s (elem _) d),(nth s' (elem _) d).
    eexists (unflatten_in _ _ v), (unflatten_acts _ _ v').
-   specialize (flatTrans_res_ok H H') as (?&?&?).
-   specialize (flatTrans_in_ok H H') as (?&?&?).
    unfold unflatten_trans.
+   specialize (flatTrans_bound H H') as (?&<-&?&?&?&?).
    rewrite !index_nth_elem_fint. 2,3:easy.
    rewrite unflatten_in_correct. 2,3:now try rewrite Card_Fint;easy.
-   erewrite lookup_sound. 3:easy. 2:eapply flatTrans_inj;eassumption.
+   erewrite lookup_sound. 2:eapply flatTrans_inj;eassumption. 2:easy.
    cbn.
    setoid_rewrite unflatten_in_correct. 2,3:now try rewrite Card_Fint;easy.
    setoid_rewrite unflatten_acts_correct. 2,3:now try rewrite Card_Fint;easy.
    repeat split.
-  -intros (?&?&?&?&H'&->&->&->&->).
-   unfold unflatten_trans in H'.
-   edestruct (proj2 (flatTrans_tot H (index x) (map (option_map index) (Vector.to_list x1) ))).
-   { repeat split.
-     -rewrite <- (Card_Fint). eapply index_le.
-     -clear. symmetry.  rewrite map_length,vector_to_list_length. reflexivity.
-     -intros ? ([]&[= <-]&?)%in_map_iff. rewrite <- (Card_Fint). eapply index_le.
-   }
-   erewrite lookup_sound in H'. 3:eassumption. 2:now eapply flatTrans_inj;eassumption.
-   destruct x3. inv H'.
-
-   specialize (flatTrans_res_ok H H0) as (?&?&?).
-   specialize (flatTrans_in_ok H H0) as (?&?&?).
-   
-   rewrite unflatten_acts_correct. 2,3:eauto.
-   rewrite index_nth_elem_fint. all:now try rewrite Card_Fint;easy.
+  -intros s0 v0.
+   unfold unflatten_trans.
+   edestruct lookup_complete with (def := (0,@nil (option nat * move))) as [H'|H'].
+   +erewrite lookup_sound. 3:eassumption. 2:eapply flatTrans_inj;eassumption.
+    edestruct lookup as (st0,l__r). left.
+    specialize (flatTrans_bound H H') as (?&?&?&?&?&?).
+    rewrite !index_nth_elem_fint. 2,3:easy. cbn in *.
+    replace ((index s0, map (option_map index) (Vector.to_list v0),
+              (st0, map (map_fst (option_map index)) (Vector.to_list (unflatten_acts (finType_CS (Fin.t sig)) n l__r)))))
+      with (index s0, map (option_map (fun x : Fin.t sig => index x)) (Vector.to_list v0), (st0, l__r)).
+    2:{ repeat f_equal. symmetry. rewrite unflatten_acts_correct. 1,2:easy. rewrite Card_Fint. easy. }
+    eassumption.
+   +erewrite lookup_sound'. 2:eapply flatTrans_inj;eassumption.
+    2:{right. easy. }
+    cbn. right.
+    setoid_rewrite index_nth. split. easy.
+    clear. unfold unflatten_acts,unflatten_acts'.
+    rewrite map_repeat. cbn.
+    (*Set Printing Implicit.*)
+    pattern n at 1 2 4 5 6 7 8.
+    replace n with (length (@repeat (option (Fin.t sig) * move) (@None (Fin.t sig), N) n)) at 1.
+    2:now rewrite repeat_length.
+    rewrite Vector_of_list_length_eq.
+    induction n;cbn. easy.
+    rewrite <- IHn. easy. 
 Qed.
 
 
 Lemma isFlatteningTrans_validFlatTrans n sig' (M' : mTM sig' n) f:
 isFlatteningTransOf f (TM.trans (m:=M'))
--> validFlatTrans (Cardinality (TM.states M')) (Cardinality sig') n f.
+-> validFlatTrans (Cardinality sig') n (Cardinality (TM.states M')) f.
 Proof.
   intros [H'].
   split.
@@ -259,66 +267,274 @@ Proof.
    +now apply vector_to_list_inj.
    +intros [] [] [=]. 2:easy.
     f_equal;eauto using injective_index.
-  -intros. split.
-   +intros ([]&(?&?&?&?&?&->&->&->&->)%H').
-    repeat split.
-    *eapply index_le.
-    *rewrite map_length,vector_to_list_length. easy.
-    *intros ? ([]&[=<- ]&?)%in_map_iff. eapply index_le.
-   +intros (?&<-&?).
-    specialize H' with (s:=s) (v0:=v).
-    pose (s0 := nth s (elem (TM.states M')) (TM.start M')).
-    pose (v0 := unflatten_in sig' (length v) v).
-    destruct (TM.trans (s0,v0)) as (s0',v0') eqn:eq.
-    exists (index s0', map (map_fst (option_map index)) (Vector.to_list v0')). rewrite H'.
-    eexists _,s0',_,v0'.
-    repeat esplit.
-    *eassumption.
-    *subst s0. now erewrite index_nth_elem.
-    *subst v0. erewrite unflatten_in_correct. all:easy.
-  -intros [] ? ? (?&?&?&?&?&->&->&->&->)%H'.
-   rewrite map_length. repeat split.
+  -intros. eapply H' in H as (?&?&?&?&?&->&->&->&->).
+   repeat split.
    +eapply index_le.
-   +apply vector_to_list_length.
+   +rewrite map_length,vector_to_list_length. easy.
+   +intros ? ([]&[=<- ]&?)%in_map_iff. eapply index_le.
+   +eapply index_le.
+   +rewrite map_length,vector_to_list_length. easy.
    +intros ? ? ([[]]&[= <- <-]&?)%in_map_iff. eapply index_le.
 Qed.
 
 Lemma unflattenTM_correct M:
-  (exists sig n (M' : mTM sig n), isFlatteningTMOf M M')
+  validFlatTM M
   -> isFlatteningTMOf M (unflattenTM M).
 Proof.
-  intros (sig'&n&M'&H). destruct M. inv H.
-  assert (H_st:(Init.Nat.max 1 states) = states).
-  {destruct states. 2:easy.
-   exfalso.
-   enough (TM.start M' el []) by easy.
-   unfold Cardinality in eq__states.
-   symmetry in eq__states. eapply length_zero_iff_nil in eq__states.
-   rewrite <- eq__states.
-   eapply elem_spec.
-  }
-  cbn - [max] in *.
+  intros (?&?). destruct M.
+  cbn in *.
+  assert (H_st:(Init.Nat.max 1 states) = states) by now destruct states.
   econstructor; cbn - [max].
   -easy.
   -now rewrite Card_Fint.
-  -cbn - [Cardinality max].
-   rewrite H_st.
+  -rewrite H_st.
    setoid_rewrite <- Card_Fint at 1. easy.
   -eapply unflatten_trans_correct. 
-   rewrite H_st. subst states sig.
-   eapply isFlatteningTrans_validFlatTrans. easy.
-  -cbn -[max].
-   generalize (def states).
+   rewrite H_st. easy.
+  -generalize (def states).
    rewrite H_st. intros ?.
    unfold index. setoid_rewrite getPosition_nth. easy.
    +apply dupfree_elements.
-   +rewrite eq__start, eq__states.
-    refine (_:_ < Cardinality _).
-    setoid_rewrite Card_Fint at 1.
-    unfold Cardinality.
-    eapply index_le.
-  -cbn -[max unflatten_trans]. rewrite H_st.
+   +refine (_:_ < Cardinality _).
+    setoid_rewrite Card_Fint at 1. easy.
+  -cbn -[max]. rewrite H_st.
    econstructor. reflexivity.
 Qed.
 
-Print Assumptions unflattenTM_correct.
+Lemma isFlattening_is_valid M sig n (M':mTM sig n):
+  isFlatteningTMOf M M'
+  -> validFlatTM M.
+Proof.
+  intros []. destruct M.
+  cbn in *;subst.
+  split;cbn.
+  -now apply isFlatteningTrans_validFlatTrans.
+  -apply index_le.
+Qed.
+
+Definition allSameEntry {X Y} (eqbX:X -> X -> bool) (eqbY:Y -> Y -> bool) x y (f : list (X*Y)) :=
+  forallb (fun '(x',y') => implb (eqbX x x') (eqbY y y')) f.
+
+Fixpoint isInjFinfuncTable {X Y} (eqbX:X -> X -> bool) (eqbY:Y -> Y -> bool) (f : list (X*Y)) :=
+  match f with
+    [] => true
+  | (x,y)::f => allSameEntry eqbX eqbY x y f
+              && isInjFinfuncTable eqbX eqbY f
+  end.
+
+Lemma allSameEntry_spec X Y eqbX eqbY x y f:
+  (forall x y : X, reflect (x = y) (eqbX x y))
+  -> (forall x y : Y, reflect (x = y) (eqbY x y))
+  -> reflect (forall (y' : Y), (x, y') el f -> y = y') (allSameEntry eqbX eqbY x y f).
+Proof.
+  intros Hx Hy. unfold allSameEntry.
+  apply iff_reflect. rewrite forallb_forall.
+  transitivity (forall x' y',  (x',y') el f -> implb (eqbX x x') (eqbY y y') = true).
+  2:{split. now intros ? [].
+     intros H x' y'. specialize (H (x',y'));cbn in H. easy. }
+  split.
+  -intros H x' y' ?.
+   destruct (Hx x x'). 2:easy.
+   edestruct (Hy y y') as [ | []]. easy.
+   subst. eauto.
+  -intros H y' ?.
+   specialize (H x y').
+   destruct (Hx x x). 2:easy.
+   edestruct (Hy y y') as [ | ]. easy.
+   apply H in H0. easy.
+Qed.
+
+Lemma isInjFinfuncTable_spec X Y eqbX eqbY f:
+  (forall x y : X, reflect (x = y) (eqbX x y))
+  -> (forall x y : Y, reflect (x = y) (eqbY x y))
+  -> reflect (forall (a : X) (b b' : Y), (a, b) el f -> (a, b') el f -> b = b') (isInjFinfuncTable eqbX eqbY f).
+Proof.
+  intros Hx Hy. induction f as [ |[x y] f].
+  cbn;constructor. easy.
+  cbn.
+  edestruct (allSameEntry_spec x y f Hx Hy) as [H' | H'].
+  2:{cbn. constructor.
+     intros H. eapply H'.  intros.
+     eapply H;[left|right].  all:easy.
+  }
+  cbn.
+  eapply ssrbool.equivP. eassumption.
+  split. 2:now firstorder.
+  intros ? ? ? ? [[= -> ->]| ] [[= ->] | ]. all:subst.
+  3:symmetry. all:easy.
+Qed.           
+
+Print validFlatTrans.
+
+Definition isBoundTransTable (sig n states : nat) (f : list (nat * list (option nat) * (nat * list (option nat * move)))) :=
+  forallb (fun '((s,v),(s',v')) =>
+             (s <? states)
+               && (length v =? n)
+               && (forallb (fun a => match a with None => true | Some a => a <? sig end) v)
+               && (s' <? states)
+               && (length v' =? n)
+               && (forallb (fun a => match fst a with None => true | Some a  => a <? sig end) v')) f.
+
+Lemma isBoundTransTable_spec sig n states f:
+  reflect (forall (s s' : nat) (v : list (option nat)) (v' : list (option nat * move)),
+              (s, v, (s', v')) el f ->
+              s < states /\
+          | v | = n /\
+                (forall a : nat, Some a el v -> a < sig) /\
+                s' < states /\ | v' | = n /\ (forall (a : nat) (m : move), (Some a, m) el v' -> a < sig))
+          (isBoundTransTable sig n states f).
+Proof.
+  unfold isBoundTransTable.
+  apply iff_reflect. rewrite forallb_forall.
+  transitivity (forall (s s' : nat) (v : list (option nat)) (v' : list (option nat * move)),
+                    (s, v, (s', v')) el f 
+     -> (((s <? states) && (| v | =? n) && forallb (fun a : option nat => match a with
+                                                                     | Some a => a <? sig
+                                                                     | None => true
+                                                                     end) v && (s' <? states) && (| v' | =? n) &&
+     forallb (fun a : option nat * move => match fst a with
+                                           | Some a => a <? sig
+                                           | None => true
+                                      end) v') = true)).
+  2:{split. now intros H [[] []]. 
+     intros H s s' v v'. specialize (H ((s,v),(s',v')));cbn in H. easy. }
+  do 4 (eapply Morphisms_Prop.all_iff_morphism;intros ?).
+  eapply Morphisms_Prop.iff_iff_iff_impl_morphism. easy.
+  rewrite <- !andb_assoc. rewrite !andb_true_iff. 
+  repeat apply Morphisms_Prop.and_iff_morphism.
+  1,4:now rewrite Nat.ltb_lt.
+  1,3:now rewrite Nat.eqb_eq.
+  all:rewrite forallb_forall.
+  {split.
+   -intros ? []. rewrite Nat.ltb_lt. all:easy.
+   -intros H ? ?%H. now rewrite <- Nat.ltb_lt.
+  }
+  {split.
+   -intros ? [[] ]; cbn - [Nat.ltb]. rewrite Nat.ltb_lt. all:easy.
+   -intros H ? ? ?%H. now rewrite <- Nat.ltb_lt.
+  }
+Qed.   
+
+Definition isValidFlatTrans sig n states (f : list (nat * list (option nat) * (nat * list (option nat * move)))) :=
+  isInjFinfuncTable (LProd.prod_eqb Nat.eqb (Lists.list_eqb (LOptions.option_eqb Nat.eqb)))
+                    (LProd.prod_eqb Nat.eqb (Lists.list_eqb (LProd.prod_eqb (LOptions.option_eqb Nat.eqb) TMEncoding.move_eqb))) f && isBoundTransTable sig n states f.
+
+Lemma isValidFlatTrans_spec sig n states f:
+  reflect (validFlatTrans sig n states f)
+          (isValidFlatTrans sig n states f).
+Proof.
+  unfold isValidFlatTrans.
+  eapply iff_reflect.
+  rewrite andb_true_iff. rewrite <- !reflect_iff.
+  2:{ eapply isBoundTransTable_spec. }
+  2:{ eapply isInjFinfuncTable_spec.
+      all:intros;eauto using LProd.prod_eqb_spec, LOptions.option_eqb_spec, Lists.list_eqb_spec, TMEncoding.move_eqb_spec, Nat.eqb_spec. }
+  split.
+  -now intros [].
+  -econstructor. all:easy.
+Qed.
+
+Definition isValidFlatTM M :=
+  isValidFlatTrans M.(sig) M.(tapes) M.(states) M.(trans) && (M.(start) <? M.(states)).
+
+Lemma isValidFlatTM_spec M:
+  reflect (validFlatTM M)
+          (isValidFlatTM M).
+Proof.
+  unfold isValidFlatTM.
+  eapply iff_reflect.
+  destruct M; cbn -[Nat.ltb].
+  rewrite andb_true_iff. rewrite <- !reflect_iff.
+  2:{ apply Nat.ltb_spec0. }
+  2:{ apply isValidFlatTrans_spec. }
+  split;intros []. all:easy.
+Qed.
+
+(** ** unflatten Tapes *)
+
+Definition isValidFlatTape (sig:nat) (t:tape nat):=
+  forallb (fun x => Nat.ltb x sig) (tapeToList t).
+
+Definition isValidFlatTapes (sig:nat) n (t:list (tape nat)):=
+  (length t =? n) && forallb (isValidFlatTape sig) t.
+
+Lemma tapeToList_map_commute sig sig' (f : sig -> sig') t :
+  tapeToList (mapTape f t) = map f (tapeToList t).
+Proof.
+  destruct t;cbn. all:simpl_list.
+  all:try rewrite !map_rev. all:easy.
+Qed.
+
+Lemma flatteningTapeIsValid (sig:finType) n t (t' : TM.tapes sig n):
+  isFlatteningTapesOf t t' ->
+  isValidFlatTapes (Cardinality.Cardinality sig) n t = true.
+Proof.
+  intros H. inv H.
+  unfold isValidFlatTapes.
+  rewrite andb_true_iff. split.
+  {rewrite vector_to_list_length. rewrite Nat.eqb_refl. easy. }
+  induction t' as [ |t];cbn. easy.
+  rewrite andb_true_iff. split.
+  2:{easy. }
+  unfold isValidFlatTape.
+  rewrite tapeToList_map_commute.
+  setoid_rewrite forallb_forall.
+  intros ? (?&?&?)%in_map_iff.
+  rewrite Nat.ltb_lt.
+  subst. eapply index_le.
+Qed.
+
+
+Lemma isUnflattableTape sig t:
+  isValidFlatTape (Cardinality sig) t = true -> {t' & t = (mapTape (index (F:=sig)) t')}.
+Proof.
+  cbn. unfold isValidFlatTape.
+  intros H. rewrite forallb_forall in H. setoid_rewrite Nat.ltb_lt in H.
+  destruct t;cbn - [Nat.ltb].
+  -exists (niltape _). easy.
+  -eexists (leftof _ _). cbn. f_equal.
+   +symmetry;eapply index_nth_elem. apply H. cbn;easy.
+   +erewrite utils.map_map_compose. erewrite map_ext_in. now rewrite map_id.
+    intros. cbn. unfold Basics.compose. eapply index_nth_elem. apply H. cbn;easy.
+  -eexists (rightof _ _). cbn. f_equal.
+   +symmetry;eapply index_nth_elem. apply H. cbn;easy.
+   +erewrite utils.map_map_compose. erewrite map_ext_in. now rewrite map_id.
+    intros. cbn. unfold Basics.compose. eapply index_nth_elem. apply H. cbn. rewrite in_app_iff, <- in_rev. eauto. 
+  -eexists (midtape _ _ _). cbn. f_equal.
+   +erewrite utils.map_map_compose. erewrite map_ext_in. now rewrite map_id.
+    intros. cbn. unfold Basics.compose. eapply index_nth_elem. apply H. cbn. rewrite in_app_iff, <- in_rev. eauto. 
+   +symmetry;eapply index_nth_elem. apply H. cbn;easy.
+   +erewrite utils.map_map_compose. erewrite map_ext_in. now rewrite map_id.
+    intros. cbn. unfold Basics.compose. eapply index_nth_elem. apply H. cbn. rewrite in_app_iff, <- in_rev. eauto.
+    Unshelve.
+    all:cbn in H.
+    all:eapply defFin.
+    all:eapply Nat.le_lt_trans;[ | eapply H;easy].
+    all:Lia.lia.
+Qed.
+    
+   
+Lemma isUnflattableTapes sig n t :
+  isValidFlatTapes (Cardinality sig) n t = true -> {t' & isFlatteningTapesOf (sig:=sig) (n:=n) t t'}.
+Proof.
+  cbn. unfold isValidFlatTapes.
+  intros H. rewrite !andb_true_iff in H.
+  destruct H as (H'&H).
+  eapply Nat.eqb_eq in H'. subst n.
+  induction t.
+  -eexists [||]. rewrite isFlatteningTapesOf_iff. easy.
+  -cbn in H.
+   rewrite !andb_true_iff in H. destruct H as (H'&H).
+   apply IHt in H as (v'&Hv).
+   apply isUnflattableTape in H' as (t0&Ht0).
+   eexists (t0:::v').
+   rewrite isFlatteningTapesOf_iff in *. cbn. f_equal. all: now cbv.
+Qed.
+(*
+Lemma isValidFlatTapes_spec sig n t :
+  reflect (forall sig, Cardinality sig = n -> exists t', isFlatteningTapesOf (sig:=sig) (n:=n) t t') (isValidFlatTapes (Cardinality sig) n t).
+Proof.
+  eapply iff_reflect. split.
+  -intros (?&?%flatteningTapeIsValid).  easy.
+  -intros (?&?)%isUnflattableTapes.  eauto.
+Qed.*)
