theories/L/Complexity/Problems/TMGenericNPcompleteProblem.v
@@ -1,5 +1,5 @@
 From Undecidability.TM Require Import TM.
-From Undecidability.L.TM Require Import TMflat TMflatEnc TMflatFun TMEncoding TapeDecode.
+From Undecidability.L.TM Require Import TMflat TMflatEnc TMflatFun TMEncoding TapeDecode TMunflatten.
 From Undecidability.L.Datatypes Require Import LNat LProd Lists.
 
 
@@ -15,7 +15,47 @@ Definition TMgenericNPcompleteProblem: TM*nat*nat -> Prop:=
 From Undecidability.L.Complexity Require Import NP LinTimeDecodable.
 From Undecidability.L Require Import Tactics.LTactics Functions.Decoding TMflatFun.
 
+Instance term_nat_max :
+  computableTime' (Nat.max) (fun x _ => (5,fun y _ => (min x y * 15 + 8,tt))).
+Proof.
+  extract. solverec.
+Qed.
 
+
+Instance term_tapeToList sig {H:registered sig}:
+  computableTime' (@tapeToList sig) (fun t _ => (sizeOfTape t*29 + 26,tt)).  
+extract. solverec. all:repeat simpl_list;cbn -[plus mult]. all:solverec.
+Proof.
+Qed.
+
+Instance term_length X {H:registered X}:
+  computableTime' (@length X) (fun t _ => (length t * 11 + 8,tt)).  
+extract. solverec.
+Proof.
+Qed.
+
+Instance term_sizeOfTape sig {H:registered sig}:
+  computableTime' (@sizeOfTape sig) (fun t _ => (sizeOfTape t*40 + 35,tt)).
+Proof.
+  extract. unfold sizeOfTape. solverec.
+Qed.
+
+
+Instance term_sizeOfmTapesFlat sig {H:registered sig}:
+  computableTime' (@sizeOfmTapesFlat sig) (fun t _ => (sumn (map (@sizeOfTape _) t) * 55 + length t * 58 + 8,tt)).
+Proof.
+  assert (H' : extEq
+                 (fix sizeOfmTapesFlat (ts : list (tape sig)) : nat :=
+                    match ts with
+                    | [] => 0
+                    | t :: ts0 => Init.Nat.max (sizeOfTape t) (sizeOfmTapesFlat ts0)
+                    end) (sizeOfmTapesFlat (sig:=sig))).
+  { intros x. induction x;hnf;cbn. all:easy. }
+  cbn [extEq] in H'.
+  
+  eapply computableTimeExt. exact H'.
+  extract. solverec. 
+Qed.
 
 Lemma inNP_TMgenericNPCompleteProblem:
   inNP TMgenericNPcompleteProblem.
@@ -31,7 +71,7 @@ Proof.
    exists f'. repeat eapply conj.
    {
      eexists (fun '((M,maxSize,steps),t) =>
-                if negb (sizeOfmTapesFlat t <=? maxSize)
+                if negb ((sizeOfmTapesFlat t <=? maxSize) && isValidFlatTM M && isValidFlatTapes M.(sig) M.(tapes) t)
                 then false
                 else match loopMflat M (M.(start),t) steps with
                        Some _ => true
@@ -39,11 +79,22 @@ Proof.
                      end).
      repeat eapply conj.
      2:{intros [[[M maxSize] steps] t]. cbn.
-        destruct (Nat.leb_spec0 (sizeOfmTapesFlat t) (maxSize));cbn [negb].
+        destruct (Nat.leb_spec0 (sizeOfmTapesFlat t) (maxSize));cbn [negb andb].
         2:{ split. 2:easy.
             intros (?&?&?&?&?&?&?&?). erewrite sizeOfmTapesFlat_eq in n. 2:easy. easy.
         }
+        destruct (isValidFlatTM_spec M);cbn [negb andb].
+        2:{ split. 2:easy.
+            intros (?&?&?&?&?&?&?&?). eauto using isFlattening_is_valid.
+        }
+        destruct isValidFlatTapes eqn:eq;cbn [negb andb].
+        2:{ split. 2:easy.
+            intros (?&?&?&[]&?&?&?&?). destruct M;cbn in *;subst. 
+            eapply flatteningTapeIsValid in H. easy.
+        }
         specialize loopMflat_correct with (M:=M) (c:=(M.(start),t)) (k:=steps) as H.
+        rewrite <- Card_Fint with (n:=sig M) in eq.
+        eapply unflattenTM_correct in v.
         split.
         -intros (?&?&M'&?&?&?&?&?).
          specialize H with (1:=H0) (2:=initFlat_correct H0 H1).
@@ -51,18 +102,37 @@ Proof.
          destruct loopMflat,loopM.
          all:try easy.
         -destruct loopMflat. 2:easy. intros _.
-         
-         
-        term+)
+         eexists _,_,(unflattenTM M).
+         split. now eauto using unflattenTM_correct.
+         eapply isUnflattableTapes in eq as (t'&?).
+         exists t'. split. easy.
+         specialize H with (1:=v). split. 2:now erewrite <- sizeOfmTapesFlat_eq.
+         specialize H with (c'                          :=initc (unflattenTM M) t').
+         assert (H':isFlatteningConfigOf (start M, t) (initc (unflattenTM M) t')).
+         {eapply initFlat_correct;easy. }
+         apply H in H'. destruct loopM. 2:easy.
+         eauto.
      }
-     all:admit.
+     eexists.
+
+(*
+     Instance term_allSameEntry X Y {HX:registered X} {HY:registered Y}:
+       computableTime' (@allSameEntry X Y) (fun _ t__X => (1,fun _ t__Y => (1, fun x _ => (1, fun y _ => (1,fun f _ => (cnst 0,tt)))))).
+     Proof.
+       extract. *)
+     
+     Print allSameEntry.
+     Print isInjFinfuncTable.
+     Print isValidFlatTrans.
+     Print isValidFlatTM.
+     Fail now extract. all:admit. 
    }
    all:admit.
   -evar (f:nat -> nat).
    exists f. repeat eapply conj.
    2:{
      intros [[TM maxSize] steps] y.
-     intros (?&?&?&?&R__tapes&?&?).
+     intros (?&?&?&?&?&R__tapes&?&?).
      remember (size (enc (TM, maxSize, steps))) as n eqn:Hn.
      rewrite size_flatTapes. 2:eassumption.
      rewrite !size_prod,size_TM in Hn.
